next_alt subst in dead case

theories/elpi_equiv.v
@@ -8,13 +8,429 @@ Module NurEqiv (U : Unif).
 
   Module NurP := NurProp(U).
   Import NurP Nur VS RunP Run Language.
-  Lemma same_subst (s1 s2: Sigma): s1 = s2. Admitted.
+
+  Definition set_new_subst s1 l :=
+    match l with
+    | no_alt => no_alt
+    | more_alt (_,x) xs => (s1, x) ::: xs
+    end.
+
+  (* Lemma topotip A s1 s2 s3 s4 E l x xs:
+    valid_state A ->
+    success A -> next_alt s1 A = Some (s2, E) ->
+      state_to_list E s3 l = more_alt (s4, x) xs ->
+        s3 = s4.
+  Proof.
+    elim: A s1 s2 s3 s4 E l x xs => //=.
+    - move=> A HA s B HB s1 s2 s3 s4 E l x xs.
+      case: ifP => //[dA vB sB|dA /andP[vA bB]sA].
+        case N: next_alt => [[s5 B']|]//[??]; subst => /=.
+        rewrite state_to_list_dead//=.
+        case X: state_to_list => //=[[s5 y]ys][???]; subst.
+        have:= HB _ _ _ _ _ _ _ _ vB sB N X.
+        move=> ?; subst.
+        apply: HB vB _ _ _.
+        apply: *)
+
+  Lemma s2l_bbOr_same_subst {A s1 s2 xs ys l}:
+    bbOr A -> state_to_list A s1 l = (s2, xs) ::: ys -> s1 = s2.
+  Proof.
+    move=>/orP[]; last first.
+      move=>/base_or_aux_ko_state_to_list->//.
+    case: A => //=.
+    - move=> ?[]//.
+    - move=> A s B/andP[H1 H2].
+      have [hd X]:= base_and_state_to_list H1.
+      rewrite X/= => -[???]//.
+    - move=> []//=p a _ B /andP[/eqP->]bB.
+      have [hd X]:= base_and_state_to_list bB.
+      case: a => [|t]/=; rewrite X/= => -[]//.
+  Qed.
+
+  Lemma get_substS_base_and_ko {A s1}:
+    base_and_ko A -> get_substS s1 A = s1.
+  Proof. elim: A s1 => //=-[]//= _ B0 _ B HB s1 /and3P[H1 H2]; apply: HB. Qed.
+
+  Lemma get_substS_base_and {A s1}:
+    base_and A -> get_substS s1 A = s1.
+  Proof. elim: A s1 => //=-[]//= _ _ _ B0 _ B HB s1 /andP[H1]; apply: HB. Qed.
+
+  Lemma get_substS_base_or_ko {A s1}:
+    base_or_aux_ko A -> get_substS s1 A = s1.
+  Proof.
+    elim: A s1 => //=.
+    - move=> A HA s B HB s1 /andP[H1 H2].
+      rewrite base_and_ko_is_dead//get_substS_base_and_ko//.
+    - move=> []//= _ B0 _ B HB s1 /and3P[_ _]; apply: get_substS_base_and_ko.
+  Qed.
+
+  Lemma get_substS_base_or {A s1}:
+    base_or_aux A -> get_substS s1 A = s1.
+  Proof.
+    elim: A s1 => //=.
+    - move=> A HA s B HB s1 /andP[H1 H2].
+      rewrite base_and_is_dead// get_substS_base_and//.
+    - move=> []//= _ _ _ B0 _ B HB s1 /andP[_]; apply: get_substS_base_and.
+  Qed.
+
+  Lemma get_substS_base_bbOr {A s1}:
+    bbOr A -> get_substS s1 A = s1.
+  Proof. move=>/orP[/get_substS_base_or|/get_substS_base_or_ko]//. Qed.
+
+  Lemma get_substS_next_alt_success {A A' s1 s2 s3 s4 l xs ys}:
+    valid_state A -> success A -> 
+      next_alt s1 A = Some (s2, A') -> 
+        state_to_list A' s3 l = (s4, xs) ::: ys ->
+          get_substS s3 A' = s4.
+  Proof.
+    elim: A A' s1 s2 s3 s4 l xs ys => //=.
+    - move=> A HA s B HB C s1 s2 s3 s4 l xs ys.
+      case: ifP => [dA vB sB|dA/andP[vA bB] sA].
+        case X: next_alt => //[[s5 D]][??]/=; subst.
+        move=> /=.
+        rewrite state_to_list_dead//.
+        case Y : state_to_list => //[[s5 E] l1]/= [? H ?]; subst.
+        rewrite dA.
+        move: Y; fConsA (s4, E) l1 => Y.
+        apply: HB vB sB X Y.
+      case X: next_alt => [[s5 D]|].
+        move=>[??]; subst => /=.
+        rewrite (next_alt_dead X).
+        have [fD _] := next_alt_failed X.
+        set Y:= state_to_list B _ _.
+        have [[s5 E] [l1 H]]:= failed_state_to_list (valid_state_next_alt vA X) fD s3 Y.
+        rewrite H => -[???]; subst.
+        apply: HA vA sA X H.
+      case: ifP => // _.
+      case Y: next_alt => //[[s5 D]][??]/=; subst => /=.
+      rewrite (state_to_list_dead) is_dead_dead//.
+      have [fD _] := next_alt_failed Y.
+      have [[s5 E] [l1 H]]:= failed_state_to_list (valid_state_next_alt (bbOr_valid bB) Y) fD s nilC.
+      rewrite H => -[???]; subst.
+      have bD := bbOr_next_alt_Some bB Y.
+      rewrite (s2l_bbOr_same_subst bD H).
+      have:= get_substS_base_bbOr bD.
+      move=>->//.
+    - move=> A HA B0 _ B HB C s1 s2 s3 s4 l xs ys /and5P[_ vA _] + +/andP[sA sB].
+      rewrite success_failed// success_is_dead//sA/= => vB bB.
+      case X: next_alt => [[s5 D]|].
+        move=>[??]; subst => /=.
+        rewrite (success_state_to_list)//=.
+        have [H|[hd [H H1]]]:= bbAnd_state_to_list bB; rewrite H//=.
+          case Y: state_to_list => //[[s5 xs']ys'][???]; subst.
+          apply: HB vB sB X Y.
+        have [fD _]:= next_alt_failed X.
+        set Y:= make_lB0  _ _.
+        have [[s5 E] [l1 H2]]:= failed_state_to_list (valid_state_next_alt vB X) fD (get_substS s3 A) (Y++l).
+        rewrite H2 => -[???]; subst.
+        apply: HB vB sB X H2.
+      case Y: next_alt => [[s5 D]|]//=; case: ifP => //fB.
+      move: bB => /orP[]H; last first.
+        rewrite base_and_ko_failed// in fB.
+      move=> [??]; subst => /=.
+      case Z: state_to_list => //[[s5 xs']ys'].
+      have [hd H1]:= base_and_state_to_list H.
+      rewrite H1/=H1 => -[]???; subst.
+      rewrite get_substS_base_and//.
+      apply: HA vA sA Y Z.
+  Qed.
+
+  Lemma clean_successP {s1 s2 s3 A B l}:
+    valid_state A -> success A ->
+      next_alt s1 A = Some (s2, B) -> 
+        state_to_list (clean_success A) s3 l = state_to_list B s3 l.
+  Proof.
+    elim: A s1 s2 s3 B l => //.
+    - move=> A HA s B HB s2 s3 s4 C l/=.
+      case: ifP => //[dA vB sB|dA /andP[vA bB] sA].
+        case Y: next_alt => [[s6 E]|]//[_<-]/=.
+        rewrite !(state_to_list_dead dA)/=.
+        rewrite (HB _ _ _ _ _ vB sB Y)//.
+      case nA: next_alt => [[s6 E]|].
+        move=>[_<-]/=.
+        rewrite (HA _ _ _ _ _ vA sA nA)//.
+      have H := success_next_alt_state_to_list vA sA nA.
+      case : ifP => //dB.
+      case nB: next_alt => //[[s6 E]][Hz<-]/=.
+      rewrite !add_ca_deep_cat; f_equal.
+        rewrite (state_to_list_dead is_dead_dead)/=.
+        rewrite (state_to_list_empty_clean vA sA (H empty _))//.
+      move: bB; rewrite /bbOr => /orP[] bB; last first.
+        by rewrite (next_alt_aux_base_or_ko bB) in nB.
+      subst; rewrite (base_or_aux_next_alt_some bB nB)//.
+    - move=> A HA B0 _ B HB s2 s3 s4 C l/= /and5P[_ vA _] + + /andP[sA sB].
+      rewrite sA/==>vB bB0.
+      rewrite success_is_dead//success_failed//.
+      case nB: next_alt => [[s7 E]|].
+        move=>[_<-]/=.
+        rewrite !(success_state_to_list vA sA)/=.
+        have {}HB := (HB _ _ _ _ _ vB sB nB).
+        by have [H|[hd[H H1]]]:= bbAnd_state_to_list bB0; rewrite H//=HB//.
+      case nA': next_alt => [[s7 A']|]//.
+      case: ifP => // fB0.
+      move=> [??]; subst => /=.
+      move: bB0; rewrite /bbAnd => /orP[bB|]; last first.
+        move=>/base_and_ko_failed; rewrite fB0//.
+      have [x Hb]:= base_and_state_to_list bB.
+      have {}HA := HA _ _ _ _ _ vA sA nA'. 
+      have H := success_next_alt_state_to_list vB sB nB.
+      have H1 := success_state_to_list vB sB.
+      rewrite (success_state_to_list vA sA) HA Hb/=.
+      set m:= make_lB0 _ _.
+      have:= H1 s4 (m ++ l) => /(_ _ IsList_alts).
+      rewrite H.
+      case X: state_to_list => //= _.
+      rewrite /m.
+      rewrite (state_to_list_empty_clean vB sB (H empty _)).
+      case Y: state_to_list => [|[s5 t] ts]//.
+      move: Y; fConsA (s5, t) ts => Y.
+      rewrite Hb//=.
+  Qed.
+
+  Lemma expand_failure_next_alt_state_to_list_cons {s A B s1 s2 s3 C l}:
+    valid_state A -> 
+      expand s A = Failure B ->
+        next_alt s2 B = Some (s1, C) -> 
+          state_to_list A s3 l = state_to_list C s3 l.
+  Proof.
+    elim: A s B s1 s2 s3 C l => //.
+    - move=> /= ???????? [<-]//.
+    - move=> p [|t]//.
+    - move=> A HA s B HB /= s1 C s2 s3 s4 D l.
+      case: ifP => [dA vB|dA /andP[vA bB]].
+        case eB: expand => // [B'] [<-]/=; rewrite dA.
+        case nB': next_alt => [[s5 F]|]//[_<-]/=.
+        rewrite 2!(state_to_list_dead dA) (HB _ _ _ _ _ _ _ vB eB nB')//dA//.
+      case eA: expand => //[A'][<-]/=; rewrite (expand_not_dead dA eA).
+      case nA': next_alt => [[s5 F]|].
+        move=>[_<-]/=.
+        have ->// := HA _ _ _ _ _ _ _ vA eA nA'.
+      case: ifP => dB //.
+      case nB: next_alt => //[[s5 F]][?<-]; subst.
+      move/orP: bB => []bB; last first.
+        rewrite next_alt_aux_base_or_ko// in nB.
+      rewrite !add_ca_deep_cat; f_equal.
+      rewrite (expand_failure_next_alt_none_empty vA eA nA')//=.
+      rewrite (state_to_list_dead is_dead_dead)/=.
+      rewrite (base_or_aux_next_alt_some bB nB)//.
+    - move=> A HA B0 _ B HB s C/= s2 s3 s4 D l /and5P[oA vA aB].
+      case eA: expand => //[A'|s1 A'].
+        rewrite (expand_not_solved_not_success eA erefl) (expand_failure_failed eA)/=.
+        move=> /eqP-> bB[<-]/=.
+        case: ifP => //dA.
+        rewrite (expand_failure_failed eA).
+        case nA': next_alt => //[[s5 E]].
+        case: ifP => //fB[_<-]/=.
+        move: bB; rewrite /bbAnd.
+        case Z:base_and_ko.
+          rewrite base_and_ko_failed// in fB.
+        rewrite orbF => bB.
+        have [x ->]:= base_and_state_to_list bB.
+        rewrite (HA _ _ _ _ _ _ _ vA eA nA')//.
+      have [??] := (expand_solved_same eA); subst.
+      have [sA _] := (expand_solved_success eA).
+      rewrite sA/= => vB bB0.
+      rewrite (success_state_to_list vA sA).
+      case eB: expand => //[B'][<-]/=; clear C.
+      rewrite success_is_dead// success_failed//.
+      case nB' : next_alt => [[s5 E]|].
+        move=>[_<-]/=.
+        have {}HB := HB _ _ _ _ _ _ _ vB eB nB'.
+        rewrite (success_state_to_list vA sA)/=.
+        move:bB0 => /orP[]bB; last first.
+          rewrite base_and_ko_state_to_list//HB//.
+        have [hd H]:= base_and_state_to_list bB.
+        have H1 := base_and_empty_ca bB H.
+        rewrite H/= HB//.
+      have H := expand_failure_next_alt_none_empty vB eB nB'.
+      case nA': next_alt => [[s5 E]|]//.
+      case: ifP => //fB0[?<-]; subst.
+      move: bB0; rewrite/bbAnd => /orP[]; last first.
+        move=>/base_and_ko_failed; rewrite fB0//.
+      move=> bB0.
+      have [y H1] := base_and_state_to_list bB0.
+      rewrite H1 H/=H1.
+      have H2 := clean_successP _ sA nA'.
+      rewrite H2//.
+      rewrite make_lB01_empty2 H/= cat0s.
+      case SA: state_to_list => [|[s6 x] xs]//=.
+      rewrite H1// /make_lB0/make_lB01/=!map_cons.
+  Qed.
+
+  Lemma expandedb_failure_next_alt_state_to_list_cons {s1 s2 A B C b1}:
+    valid_state A -> expandedb s1 A (Failed B) b1 -> 
+      next_alt None B = Some (s2, C) -> state_to_list_cons C -> 
+        state_to_list_cons A.
+  Proof.
+    remember (Failed _) as f eqn:Hf => + HA.
+    elim: HA s2 B C Hf; clear => //.
+    - move=> s A B HA s1 _ C [<-] vA HB sC s2 l.
+      have [x[xs {}sC]]:= sC s2 l.
+      rewrite (expand_failure_next_alt_state_to_list_cons _ HA HB)// sC.
+      by do 2 eexists.
+    - move=> s s' r A B b HA HB IH s2 C D? vA HC sD; subst.
+      have{}IH := IH _ _ _ erefl (valid_state_expand vA HA) HC sD.
+      apply: expand_state_to_list_cons vA HA notF.
+    - move=> s s' r A B b HA HB IH s2 C D? vA HC sD; subst.
+      have{}IH := IH _ _ _ erefl (valid_state_expand vA HA) HC sD.
+      apply: expand_state_to_list_cons vA HA notF.
+  Qed.
+
+  (*Lemma failed_next_alt_none_state_to_list {s s1 A}:
+    valid_state A -> failed A -> next_alt s1 A = None -> 
+      forall l, state_to_list A s l = nilC.
+  Proof.
+    elim: A s s1 => //.
+    - move=> A HA s B HB s1 s2 /=.
+      case: ifP => [dA vB fB|dA /andP[vA bB] fA].
+        case X: next_alt => [[s3 C]|]//.
+        move=> _ l; rewrite (HB _ _ _ _ X)// state_to_list_dead//.
+      case: ifP => dB.
+        case X: next_alt => [[s3 C]|]//.
+        move=>_ l; rewrite (HA _ _ _ _ X)//state_to_list_dead//.
+      case Y: next_alt => [[]|]// _ l.
+      rewrite (HA _ s2)//=.
+      rewrite (bbOr_next_alt_none bB Y)//.
+    - move=> A HA B0 HB0 B HB s1 s2 /=/and5P[oA vA aB].
+      case: ifP => /=[sA vB bB0|sA/eqP->].
+        rewrite success_failed//=success_is_dead// => fB.
+        case X: next_alt => [[]|]//.
+        case Y: next_alt => [[s3 C]|]//.
+          case: ifP => fB0// _ l.
+          rewrite (HB _ s2)//.
+          have:= bB0; rewrite /bbAnd.
+          case Z: base_and => //=.
+            rewrite base_and_failed// in fB0.
+          move=> bB0'.
+          have H := @next_alt_aux_base_and_ko _ empty bB0'.
+          have H1:= bbAnd_valid bB0.
+          rewrite (HB0 _ empty)//=.
+          case: state_to_list => //[[]]//.
+        move=> _ l.
+        rewrite (success_next_alt_state_to_list vA sA Y) (HB _ s2)//=.
+        have [->|[hd [-> _]]]//= := bbAnd_state_to_list bB0.
+        by rewrite (HB _ s2)//=.
+      case: ifP => //fA bB _ + l.
+      case: ifP => //dA.
+        rewrite (state_to_list_dead dA)//.
+      case X: next_alt => [[s3 C]|].
+        case:ifP => fB => //.
+        have:= bB; rewrite /bbAnd.
+        case Z: base_and => //=.
+          rewrite base_and_failed// in fB.
+        move=> bB0'.
+        have H := @next_alt_aux_base_and_ko _ empty bB0'.
+        have H1:= bbAnd_valid bB.
+        rewrite (HB _ empty)//=; case: state_to_list => //[[_] ? _]//.
+      have -> //:= HA _ _ vA fA X l.
+  Qed. *)
+
+
+  (* Lemma failed_next_alt_some_state_to_list {s1 A s2 s3 B l}:
+    valid_state A -> failed A -> next_alt s1 A = Some(s2, B) -> 
+      state_to_list A s3 l = state_to_list B s3 l.
+  Proof.
+    elim: A s1 s2 s3 B l => //.
+    - move=> A HA s B HB s1 s2 s3 C l/=.
+      case: ifP => [dA vB fB|dA /andP[vA bB] fA].
+        case X: next_alt => [[s4 D]|]//[_<-]/=.
+        rewrite !(state_to_list_dead dA)//=(HB _ _ _ _ _ vB fB X)//dA//.
+      case X: next_alt => [[s5 D]|]//.
+        move=>[_<-]/=.
+        rewrite (HA _ _ _ _ _ vA fA X)//(next_alt_dead X)//.
+      case: ifP => dB//.
+      case Y: next_alt => [[s5 D]|]//[_<-]/=.
+      rewrite (state_to_list_dead is_dead_dead)/=.
+      rewrite (failed_next_alt_none_state_to_list vA fA X)/=.
+      rewrite (bbOr_next_alt_some bB Y)//is_dead_dead//.
+      do 3 f_equal.
+      admit.
+    - move=> A HA B0 HB0 B HB s1 s2 s3 C l /=/and5P[oA vA aB].
+      case: (ifP (is_dead _)) => //dA.
+      case: ifP => /=[sA vB bB0|sA/eqP->].
+        rewrite success_failed//= => fB.
+        rewrite (success_state_to_list vA sA)/=.
+        case X: next_alt => [[s4 D]|]//.
+          move=>[_<-]/=.
+          rewrite (success_state_to_list vA sA)/=.
+          have{}HB := (HB _ _ _ _ _ _ fB X).
+          by have [H|[hd [H M]]]:= bbAnd_state_to_list bB0; rewrite H HB//=HB//.
+        case Y: next_alt => [[s4 D]|]//.
+        move: bB0 => /orP[]bB; last first.
+          rewrite base_and_ko_failed//.
+        rewrite base_and_failed// => -[_<-].
+        have [hd H]:= base_and_state_to_list bB.
+        rewrite H/=!(failed_next_alt_none_state_to_list vB fB X)/=.
+        rewrite (clean_successP vA sA Y).
+        case Z: state_to_list => [|[s5 z] zs]//=.
+        rewrite !H//=H//.
+        rewrite/make_lB0/make_lB01; rewrite !map_cons cat_cons.
+        rewrite cat0s; f_equal; f_equal.
+        admit.
+      case: ifP => //fA bB _.
+      case X: next_alt => [[s4 D]|]//.
+      case:ifP => fB => //-[_<-]/=.
+      rewrite (HA _ _ _ _ _ vA fA X)//.
+  Admitted. *)
+
+  Lemma expand_solved {s A s1 B} l:
+    valid_state A ->
+    expand s A = Success s1 B ->
+    exists x xs,
+      state_to_list A s l = (get_substS s1 A, x) ::: xs /\
+      nur s x xs s1 (state_to_list (clean_success B) s1 l).
+  Proof.
+    move=> vA /[dup] /expand_solved_same [??] H; subst.
+    do 2 eexists; split.
+      apply: success_state_to_list vA (expand_solved_success H).2.
+    apply: StopE.
+  Qed.
+
+  Lemma state_to_list_cutr_empty {A s l}:
+    valid_state A -> state_to_list (cutr A) s l = nilC.
+  Proof.
+    elim: A s l => //.
+    - move=> A HA s B HB s1 l /=; case: ifP => //[dA vB|dA /andP[vA bB]].
+        rewrite HB//state_to_list_dead//is_dead_cutr//.
+      rewrite HA//HB//VS.bbOr_valid//.
+    - move=> A HA B0 _ B HB s l /=/and3P[oA vA]; rewrite HA//.
+  Qed.
+
+  Lemma state_to_list_clean_cutl_empty {A s l}:
+    valid_state A -> success A -> state_to_list (clean_success (cutl A)) s l = nilC.
+  Proof.
+    elim: A s l => //.
+    - move=> A HA s B HB s1 l /=; case: ifP => [dA vB sB | dA /andP[vA bB] sA]/=.
+        by rewrite dA/= HB//state_to_list_dead//.
+      by rewrite is_dead_cutl//dA/= HA//state_to_list_cutr_empty//VS.bbOr_valid//.
+    - move=> A HA B0 _ B HB s l/=/and5P[oA vA aB] + +/andP[sA sB].
+      rewrite sA success_cut//= => vB bB0.
+      rewrite (success_state_to_list (valid_state_cut sA vA) (success_cut sA))/=.
+      rewrite HA => //.
+      have bB:= bbAnd_cutl bB0.
+      rewrite base_and_ko_state_to_list//=.
+      rewrite HB//.
+  Qed.
+
+  Lemma state_to_list_cutl {A s l}:
+    valid_state A -> success A -> state_to_list (cutl A) s l = (get_substS s A, nilC) ::: nilC.
+  Proof.
+    elim: A s l => //.
+    - move=> A HA s B HB s1 l /=; case: ifP => [dA vB sB | dA /andP[vA bB] sA]/=.
+        rewrite HB// state_to_list_dead//=.
+      by rewrite (state_to_list_cutr_empty (VS.bbOr_valid bB))/=cats0 HA.
+    - move=> A HA B0 _ B HB s l/=/and5P[oA vA aB] + +/andP[sA sB].
+      rewrite sA/==> vB bB0.
+      rewrite HA//.
+      have bB:= bbAnd_cutl bB0.
+      rewrite base_and_ko_state_to_list//=HB//.
+  Qed.
   
-  Lemma map_nil l:
+  (* Lemma map_nil (l: alts):
     map (appendC^~ nilC) l = l.
   Proof.
     elim: l => //=x xs H; rewrite map_cons H cats0//.
-  Qed.
+  Qed. *)
 
   Lemma save_alt_add_ca_deepA bt a gs bs:
     empty_ca bs ->
@@ -27,7 +443,7 @@ Module NurEqiv (U : Unif).
   Proof.
     all: rewrite/save_alts/save_goals/empty_ca in save_alt_add_ca_deepA save_alt_add_ca_deepG *.
     {
-      case: bs => //=b bs.
+      case: bs => //=-[s1 b] bs.
       rewrite all_cons =>/andP[H1 H2].
       rewrite map_cons.
       rewrite (save_alt_add_ca_deepG _ _ _ _ H1).
@@ -74,7 +490,7 @@ Module NurEqiv (U : Unif).
         (append_goals (add_deepG l hd tl) hd) rs.
   Proof.
     move=> H.
-    elim: rs => //=g gs IH.
+    elim: rs => //=-[s1 g] gs IH.
     rewrite /empty_ca all_cons=>/andP[H1 H2].
     rewrite/make_lB0/save_alts !map_cons; f_equal.
       rewrite add_deep_goalsP//.
@@ -89,14 +505,6 @@ Module NurEqiv (U : Unif).
     rewrite/empty_ca.
     elim: rs => //=-[s b l]/= H.
     rewrite all_cons empty_ca_atoms//.
-  Qed.
-
-  Lemma base_and_empty_top {B l}:
-    base_and B -> state_to_list B l = nilC:::nilC -> B = Top.
-  Proof.
-    elim: B l => //=-[]//=p  a _ _ _ B HB l /andP[/eqP->] bB.
-    have [hd H] := base_and_state_to_list bB.
-    case: a; rewrite/=!H//=.
   Qed.
 
   Lemma expand_cb_failedF {s1 s2 A B}:
@@ -123,7 +531,7 @@ Module NurEqiv (U : Unif).
   Qed.  
   
   Definition will_cut l :=
-    match l with more_alt (more_goals (cut _) _) _ => true | _ => false end.
+    match l with more_alt (_, more_goals (cut _) _) _ => true | _ => false end.
 
   Fixpoint will_call l ca :=
     match l with
@@ -132,8 +540,8 @@ Module NurEqiv (U : Unif).
     | more_goals (call pr t) gs => Some (pr,t,ca,gs)
     end.
 
-  Lemma s2l_big_and p1 r1 l: 
-    state_to_list (big_and p1 r1) l = (a2gs p1 r1) ::: nilC.
+  Lemma s2l_big_and p1 r1 s l: 
+    state_to_list (big_and p1 r1) s l = (s, a2gs p1 r1) ::: nilC.
   Proof. 
     elim: r1 => //=-[|t] xs H//=; rewrite H/=.
     - rewrite drop0 take0 make_lB0_empty1 !cat0s cats0.
@@ -141,113 +549,111 @@ Module NurEqiv (U : Unif).
     - rewrite make_lB0_empty1 cats0/make_lB01/= map_cons cat_cons cat0s//.
   Qed.
 
-  Lemma s2l_big_or s {p1 b bs ca gs}:
-    (save_goals ca gs (a2gs p1 b)) ::: (save_alts ca gs (aa2gs p1 bs)) =
-    map (fun x => x ++ gs) (state_to_list ((Or Bot s (big_or_aux p1 b bs))) ca).
+  Lemma s2l_big_or k s {p1 b bs ca gs}:
+    (s, save_goals ca gs (a2gs p1 b)) ::: (save_alts ca gs (aa2gs p1 bs)) =
+    make_lB0 (state_to_list ((Or Bot s (big_or_aux p1 b bs))) k ca) gs.
   Proof. 
-    move=>/=; clear s.
+    move=>/=; clear k.
     rewrite cat0s.
-    elim: bs b ca gs => //=.
-      move=> b ca gs.
-      rewrite s2l_big_and/= map_cons; f_equal.
+    elim: bs s b ca gs => //=.
+      move=> s b ca gs.
+      rewrite s2l_big_and/=/make_lB0 map_cons; f_equal.
       rewrite /save_goals; f_equal.
       have:= empty_ca_atoms p1 b.
       set X := (a2gs _ _).
       generalize X => {}X.
-      apply: add_ca_deep_goals_map.
-    move=> [s1 [hd bo]]/=rs IH b ca gs/=.
-    rewrite add_ca_deep_empty1 add_ca_deep_cat map_cat s2l_big_and/=map_cons.
+      move=> /add_ca_deep_goals_map->//.
+    move=> [s1 [hd bo]]/=rs IH s2 b ca gs/=.
+    rewrite add_ca_deep_empty1 add_ca_deep_cat /make_lB0 map_cat s2l_big_and/=map_cons.
     rewrite cat_cons cat0s; f_equal.
       rewrite -add_ca_deep_goals_map//.
       rewrite empty_ca_atoms//.
-    rewrite-IH//.
+    apply: IH.
   Qed.
 
-
-  Lemma s2l_CutBrothers {s1 A s2 B} l1:
+  Lemma s2l_CutBrothers {s1 A s2 B} sA l1:
     valid_state A -> expand s1 A = CutBrothers s2 B -> 
       exists x tl, 
-        ((state_to_list A l1 = ((cut nilC) ::: x) ::: tl) *
-          (forall l, (state_to_list B l = x ::: nilC)) * (empty_caG x))%type.
+        ((state_to_list A sA l1 = (get_substS sA A, (cut nilC) ::: x) ::: tl) *
+          (forall l sB, (state_to_list B sB l = (sB, x) ::: nilC)) * 
+            (empty_caG x))%type.
   Proof.
     move=>/=.
-    elim: A s1 s2 B l1 => //.
-    - move=> p []//= ?????[_<-]/=; by do 2 eexists.
-    - move=> A HA s B HB s1 s2 C l1 /=.
+    elim: A sA s1 s2 B l1 => //.
+    - move=> p []//= ??????[_<-]/=; by do 2 eexists.
+    - move=> A HA s B HB sA s1 s2 C l1 /=.
       by case: ifP => [dA vB|dA/andP[vA bB]]; case eB: expand => //[s1' B'][??]; subst.
-    - move=> A HA B0 _ B HB s1 s2 C l1/=/and5P[oA vA aB].
+    - move=> A HA B0 _ B HB sA s1 s2 C l1/=/and5P[oA vA aB].
       case eA: expand => //[s3 A'|s3 A'].
         rewrite (expand_not_solved_not_success eA erefl)/=(expand_not_failed eA notF).
         move=>/eqP->bB [_<-]/=.
         have [y  H1] /=:= base_and_state_to_list bB.
-        have [x [tl [[H3 H4] H5]]] := HA _ _ _ l1 vA eA.
+        have {HA}[x [tl [[H3 H4] H5]]] := HA sA _ _ _ l1 vA eA.
         have /= H6 := base_and_empty_ca bB H1.
-        rewrite H1 H3/= cats0/= size_nil take0 make_lB0_empty1 H1/=.
-        rewrite/make_lB01/make_lB0/map/appendC/=.
-        do 2 eexists; split.
-          split => //.
-          move=> l; rewrite H4 H1/=H1/=.
-          rewrite !empty_caG_add_deepG//.
-        rewrite !empty_caG_add_deepG///empty_caG all_cat.
-        apply/andP; split => //; apply:H6.
-      have [sA sA'] := expand_solved_success eA.
-      rewrite sA/==> vB bB0.
+        do 2 eexists; repeat split.
+        - rewrite H1 H3/= take0 drop0 make_lB0_empty1 H1 !cat_cons//(get_substS_base_and bB)//.
+        - move=> l sB; rewrite H1/= H4/=H1 cats0 empty_caG_add_deepG//empty_caG_add_deepG//.
+        - rewrite !empty_caG_add_deepG///empty_caG all_cat.
+          apply/andP; split => //; apply:H6.
+      have [sAx _] := expand_solved_success eA.
+      rewrite sAx/==> vB bB0.
       case eB: expand => //[s4 B'] [_<-]/=.
       rewrite !(expand_solved_same eA).
-      rewrite (success_state_to_list (valid_state_expand vA eA) sA')/=.
       have [??]:= expand_solved_same eA; subst.
-      have [H2|[hd[H2 H3]]] := bbAnd_state_to_list bB0; rewrite H2.
-        have [x[tl [H H1]]] := HB _ _ _ l1 vB eB.
-        rewrite H.
-        do 2 eexists; split.
-          split => //l.
-          rewrite state_to_list_cutl//.
-          rewrite (base_and_ko_state_to_list (bbAnd_cutl bB0)) H//.
-        move=>//.
-      move=>/=.
+      rewrite (success_state_to_list (valid_state_expand vA eA) sAx)/=.
+      have [H2|[hd[H2 H3]]] := bbAnd_state_to_list bB0; rewrite H2/=.
+        have {HB}[x[tl [H H1]]] := HB (get_substS sA A')  _ _ _ l1 vB eB.
+        do 2 eexists; split; try eassumption.
+        rewrite H/make_lB01 map_cons; f_equal; f_equal; split => //.
+        move=> l sb.
+        rewrite state_to_list_cutl//=.
+        rewrite (base_and_ko_state_to_list (bbAnd_cutl bB0)) H//=.
+        rewrite/make_lB01 map_cons; f_equal; f_equal.
+        admit.
       set X:= make_lB0 _ _.
-      have [x[tl [H H1]]] := HB _ _ _ (X++l1) vB eB.
-      rewrite H/= make_lB01_empty2.
-      do 2 eexists; split.
-        split => //l.
-        rewrite state_to_list_cutl//.
-        have:= bbAnd_cutl bB0.
-        move=>/base_and_ko_state_to_list->.
-        rewrite H//.
-      move=>//.
-  Qed.
+      have [x[tl [H H1]]] := HB (get_substS sA A') _ _ _ (X++l1) vB eB.
+      rewrite H//=.
+      do 2 eexists; split; try eassumption.
+      rewrite make_lB01_empty2//=cat_cons; f_equal; f_equal; split => //.
+      move=> //l sB.
+      rewrite state_to_list_cutl//.
+      have:= bbAnd_cutl bB0.
+      move=>/base_and_ko_state_to_list->/=.
+      rewrite H///make_lB01 map_cons; repeat f_equal.
+      admit.
+  Admitted.
 
-  Lemma s2l_Expanded_nil {A B s1 s2 l1 ws}: valid_state A ->
-    state_to_list A l1 = nilC ::: ws -> expand s1 A = Expanded s2 B -> 
-      ((failed B = false) * (state_to_list B l1 = nilC ::: ws) * (s1 = s2))%type.
+  Lemma s2l_Expanded_nil {A B s1 s2 s3 s4 l1 ws}: valid_state A ->
+    state_to_list A s3 l1 = (s4, nilC) ::: ws -> expand s1 A = Expanded s2 B -> 
+      ((failed B = false) * (state_to_list B s3 l1 = (s4, nilC) ::: ws) * (s1 = s2))%type.
   Proof.
-    elim: A B s1 s2 l1 ws => //; auto.
-    - move=> B s1 s2 _ xs _ _ [_<-]//.
+    elim: A B s1 s2 s3 s4 l1 ws => //; auto.
+    - move=> B s1 s2 s3 s4 _ xs _ _ [_<-]//.
     - move=> p[]//.
-    - move=> A HA s B HB C s1 s2 l1 ws/=.
+    - move=> A HA s B HB C s1 s2 s3 s4 l1 ws/=.
       case:ifP => [dA vB|dA/andP[vA bB]].
         rewrite state_to_list_dead//=.
-        case sB: state_to_list => //[[] xs]//=[?]; subst.
-        case e: expand => //[s' B'|s' B'][??]; subst; rewrite/=.
-          by rewrite !(HB _ _ _ _ _ vB sB e) /=state_to_list_dead//dA; split => //.
-        have [x[tl[H1 H2]]]:= s2l_CutBrothers nilC vB e.
-        by rewrite H1 in sB.
+        case sB: state_to_list => //[[s5 []] xs]//=[??]; subst.
+        case e: expand => //[s' B'|s' B'][??]; subst; rewrite/=dA (state_to_list_dead dA).
+          by rewrite !(HB _ _ _ _ _ _ _ vB sB e).
+        have [x[tl[H1 H2]]]:= s2l_CutBrothers s nilC vB e.
+        by rewrite H1// in sB.
       case eA: expand => //[s' A'|s' A'].
-        have [x[xs H]]:= failed_state_to_list vA (expand_not_failed eA notF) (state_to_list B nilC).
-        rewrite H; case: x H => H//=[?][??]/=; subst.
-        have {}HA := (HA _ _ _ _ _ vA H eA).
-        rewrite!HA/= (expand_not_dead dA eA) !HA//.
-      have [x[tl[H1 H2]]]:= s2l_CutBrothers ((state_to_list B nilC)) vA eA.
-      rewrite H1//=.
-    - move=> A HA B0 _ B HB C s1 s2 l1 ws/=/and5P[oA vA aB].
+        have [[s5 x][xs H]]:= failed_state_to_list vA (expand_not_failed eA notF) s3 (state_to_list B s nilC).
+        rewrite H; case: x H => H //=[??][??]; subst.
+        have {}HA := (HA _ _ _ _ _ _ _ vA H eA).
+        by rewrite!HA/= (expand_not_dead dA eA) !HA//.
+      have [x[tl[H1 H2]]]:= s2l_CutBrothers s3 ((state_to_list B s nilC)) vA eA.
+      by rewrite H1//=.
+    - move=> A HA B0 _ B HB C s1 s2 s3 s4 l1 ws/=/and5P[oA vA aB].
       case eA: expand => //[s1' A'|s1' A'].
         rewrite (expand_not_solved_not_success eA erefl)(expand_not_failed eA notF)/=.
         move=> /eqP->bB.
         have [hd H]:= base_and_state_to_list bB; rewrite H.
-        case sA: state_to_list => [|y ys]//=.
+        case sA: state_to_list => [|[s5 y] ys]//=.
         rewrite H/=; case: y sA => //sA.
-        case: hd H => //= H [?][??]; subst.
-        have {}HA := (HA _ _ _ _ _ vA sA eA).
+        case: hd H => //= H [??][??]; subst.
+        have {}HA := (HA _ _ _ _ _ _ _ vA sA eA).
         by rewrite !HA/=H/=!HA/=H; rewrite base_and_failed//andbF//.
       have [??] := expand_solved_same eA; subst.
       have [_ sA] := expand_solved_success eA.
@@ -256,58 +662,61 @@ Module NurEqiv (U : Unif).
       rewrite success_state_to_list//=.
       have [H|[hd [H H1]]] := bbAnd_state_to_list bB0; rewrite H/=.
         rewrite !make_lB01_empty2.
-        by move=> H1; rewrite !(HB _ _ _ _ _ vB H1 eB)//andbF success_failed//.
+        by move=> H1; rewrite !(HB _ _ _ _ _ _ _ vB H1 eB)//andbF success_failed//.
       set m := make_lB0 _ _ ++ _.
-      have [x[xs H2]]:= failed_state_to_list vB (expand_not_failed eB notF) m.
+      have [x[xs H2]]:= failed_state_to_list vB (expand_not_failed eB notF) (get_substS s3 A') m.
       rewrite !make_lB01_empty2.
       rewrite H2/= => -[??]; subst.
-      have H3 := HB _ _ _ _ _ vB H2 eB.
+      have H3 := HB _ _ _ _ _ _ _ vB H2 eB.
       by rewrite !H3// success_failed//sA//.
   Qed.
 
-  Lemma xxx {A l ca tl alts s r} l1:
+  Lemma xxx {A l ca tl alts s r} {s1 s2} s3 l1:
     valid_state A ->
-    state_to_list A l = (((cut ca) ::: tl) ::: alts) ->
-      expand s A = r -> size(state_to_list (get_state r) l1) <> 0.
+    state_to_list A s1 l = ((s2, ((cut ca) ::: tl)) ::: alts) ->
+      expand s A = r -> size(state_to_list (get_state r) s3 l1) <> 0.
   Proof.
     move=>++<-; clear r.
-    elim: A l l1 ca tl alts s => //=.
+    elim: A l l1 ca tl alts s s1 s2 s3 => //=.
     - move=> p[]//.
-    - move=> A HA s1 B HB l l1 ca tl alts s.
+    - move=> A HA s0 B HB l l1 ca tl alts s s1 s2 s3.
       case: ifP => //[dA vB|dA/andP[vA bB]].
         rewrite (state_to_list_dead dA)/=.
-        case SB: state_to_list => [|[|[|ca'] gs] tl']//=.
-        move=>[???]; subst.
+        case SB: state_to_list => [|[sx[|[]ca' gs tl']]]//=.
+        move=>[????]; subst.
         rewrite get_state_Or/= state_to_list_dead//=.
-        set X:= state_to_list _ _.
-        case Y: X => //.
-        have:= HB _ nilC _ _ _ s vB SB.
-        rewrite size_add_ca_deep.
-        move=> /(_ _ IsList_alts).
+        set X:= state_to_list _ _ _ .
+        case Y: X => [|[]]//=.
+        have:= HB _ nilC _ _ _ _ _ _ s0 vB SB.
+        move=> /(_ _ IsList_alts s).
         by rewrite -/X Y//.
-      have:= HB nilC _ _ _ _ _ (bbOr_valid bB).
-      set SB := state_to_list B _.
-      case SA: state_to_list => [|[|[|ca'] gs] tl']//=.
-        case SB': SB => [|[|[|ca'] gs] tl']//=.
-        move=>+[???]; subst.
-        move=> /(_ _ IsList_alts); rewrite-/SB SB'.
-        move=> -/(_ _ _ _ _ _ erefl) HH.
-        case E: expand => [s' A'|s' A'|A'|s' A']/=; rewrite-/SB ?SB' size_add_ca_deep size_cat; case: size => //.
-        have [?[?[]]]:= s2l_CutBrothers SB vA E.
+      have:= HB nilC _ _ _ _ _ _ _ _ (VS.bbOr_valid bB).
+      set SB := state_to_list B _ _.
+      case SA: state_to_list =>  [|[sx[|[]ca' gs tl']]]//=.
+        case SB': SB =>  [|[sx[|[]ca' gs tl']]]//=.
+        move=>+[????]; subst.
+        move=> /(_ _ IsList_alts _ _ _ _ _ s0); rewrite-/SB SB'.
+        move=> -/(_ _ _ _ _ _ _ _ erefl) HH.
+        case E: expand => [s' A'|s' A'|A'|s' A']/=; 
+        rewrite size_add_ca_deep size_cat -/SB?SB'?size_cons; try by lia.
+        case: size => //.
+        have [?[?[]]]:= s2l_CutBrothers s1 SB vA E.
         by move=>[]; rewrite SA//.
       move=> {}HB.
       move=>[???]; subst.
-      have := HA _ SB _ _ _ s vA SA.
-      case: expand => [s' A'|s' A'|A'|s' A']/=; rewrite-/SB ?SB' size_add_ca_deep size_cat; case X: size => //.
-      erewrite (@state_to_list_same_size_aux _ _ _ _ SB erefl erefl).
-      rewrite X//.
-    - move=> A HA B0 _ B HB l l1 ca tl alts s/and5P[_ vA _].
+      move: SA; fConsG (cut ca') gs; fConsA (s2, (cut ca') ::: gs) tl' => SA.
+      have:= HA _ SB _ _ _ s _ _ s3 vA SA.
+      case e: expand => [s' A'|s' A'|A'|s' A']/=; 
+      rewrite size_add_ca_deep size_cat -/SB ?SB'; case X: size => //[n].
+      set Y:= state_to_list (cutr B) _ _.
+      rewrite (s2l_size s3 SB) X//.
+    - move=> A HA B0 _ B HB l l1 ca tl alts s s1 s2 s3/and5P[_ vA _].
       case: ifP => //=[sA vB bB0|sA/eqP-> bB].
         rewrite success_state_to_list//.
         rewrite succes_is_solved//.
         have [H|[hd[H H1]]]:= bbAnd_state_to_list bB0; rewrite H/=.
           rewrite make_lB01_empty2.
-          move=>/(HB _ _ _ _ _ s vB).
+          move=>/(HB _ _ _ _ _ s _ _ _ vB).
           case e: expand => //= Hz; rewrite success_state_to_list//=?H?success_cut//?valid_state_cut//?size_map//.
           have:= bbAnd_cutl bB0.
           by move=>/base_and_ko_state_to_list ->; rewrite /= make_lB01_empty2//.
@@ -317,10 +726,10 @@ Module NurEqiv (U : Unif).
           case eB: expand => //=[s' B'] _.
           rewrite make_lB01_empty2.
           set X:= make_lB0 _ _.
-          have [hd1[tl1[Hz Hw]]] := s2l_CutBrothers (X ++ l) vB eB.
+          have [hd1[tl1[Hz Hw]]] := s2l_CutBrothers  (get_substS s1 A) (X ++ l) vB eB.
           rewrite !Hz/= => -[???]; subst.
-          rewrite success_state_to_list?success_cut//?valid_state_cut//=.
-          by rewrite base_and_ko_state_to_list//bbAnd_cutl//.
+          rewrite success_state_to_list?success_cut//?valid_state_cut//=Hz.
+          rewrite base_and_ko_state_to_list//=bbAnd_cutl//.
         rewrite (success_state_to_list _ sA)//= H size_cat size_map.
         set SA' := state_to_list (clean_success _) _.
         case X : state_to_list => [|r rs]/=.
@@ -329,18 +738,17 @@ Module NurEqiv (U : Unif).
           have:= f_equal size H2.
           move=>/(_ _ IsList_alts).
           rewrite /make_lB0 !size_map size_cons !size_add_deep /SA/SA'.
-          rewrite (@state_to_list_same_size_aux _ _ _ _ l1 erefl erefl).
-          by move=>->; case: state_to_list => //.
+          rewrite (s2l_size s3 l1) => ->; lia.
         rewrite make_lB01_empty2.
         move=> _ [??]; subst.
         set Y:= make_lB0 _ _.
-        have:= HB _ (Y ++ l1) _ _ _ s vB X => /(_ _ IsList_alts).
+        have:= HB _ (Y ++ l1) _ _ _ s _ _ (get_substS s3 A) vB X => /(_ _ IsList_alts).
         by case: state_to_list => //.
       have {}bB: bbAnd B.
         by move: bB; case:ifP => //; rewrite /bbAnd => _ ->//.
       have [H|[hd [H Hz]]]:= bbAnd_state_to_list bB; rewrite H/=.
-        case: state_to_list => //.
-      case SA: state_to_list => [|z zs]//; rewrite H/=.
+        case: state_to_list => [|[]]//??; rewrite H//.
+      case SA: state_to_list => [|[s4 z] zs]//; rewrite H/=.
       case: z SA => //=.
         move=> Hx.
         move=>[??]; subst.
@@ -348,74 +756,76 @@ Module NurEqiv (U : Unif).
         - have H1 := (s2l_Expanded_nil vA Hx e).
           have {H1} := f_equal size (H1.1).2.
           move=>/(_ _ IsList_alts).
-          rewrite (@state_to_list_same_size_aux _ _ _ _ l1 erefl erefl).
-          by case: state_to_list => //x xs; rewrite H//= !size_cat !size_map size_add_deep H//.
-        - have [t[ts [[]]]]:= s2l_CutBrothers l vA e.
+          rewrite (s2l_size s3 l1) => //.
+          by case: state_to_list => [|[? x] xs]//=; rewrite H//= !size_cat!size_map size_add_deep H//.
+        - have [t[ts [[]]]]:= s2l_CutBrothers s1 l vA e.
           by rewrite Hx//.
         - rewrite -(expand_failure_state_to_list_same e).
           have {Hx} := f_equal size Hx.
           move=>/(_ _ IsList_alts).
-          rewrite (@state_to_list_same_size_aux _ _ _ _ l1 erefl erefl).
-          by case: state_to_list => //=x xs; rewrite H !size_cat !size_map H//.
+          rewrite (s2l_size s3 l1).
+          by case: state_to_list => //=[[? x] xs]; rewrite H !size_cat !size_map H//.
       move=> []//ca1 l2 SA []???; subst.
-      have:= HA _ l1 _ _ _ s vA SA.
-      by case e: expand => [s' A'|s' A'|A'|s' A']/=; (try rewrite (expand_solved_success e)// in sA); 
-      case SA': state_to_list => //=[x xs]; rewrite H !size_cat !size_map size_add_deep H//.
+      have:= HA _ l1 _ _ _ s _ _ s3 vA SA.
+      case e: expand => [s' A'|s' A'|A'|s' A']/=; (try rewrite (expand_solved_success e)// in sA);
+      case SA': state_to_list => //=[[? x] xs]; rewrite H !size_cat !size_map size_add_deep H//.
   Qed.
 
-  Lemma s2l_Expanded_cut {A B s0 s1 ca x tl l1}:
+  Lemma s2l_Expanded_cut {A B s0 s1 s2 s3 ca x tl l1}:
     valid_state A -> expand s0 A = Expanded s1 B ->
-      state_to_list A l1 = (((cut ca) ::: x) ::: tl) ->
-      ((failed B = false) * (s0 = s1) * (state_to_list B l1 = (((cut ca) ::: x) ::: tl) \/
-        state_to_list B l1 ++ l1 = x ::: ca))%type.
+      state_to_list A s2 l1 = (s3, ((cut ca) ::: x)) ::: tl ->
+      ((failed B = false) * (s0 = s1) * (state_to_list B s2 l1 = ((s3, (cut ca) ::: x) ::: tl) \/
+        state_to_list B s2 l1 ++ l1 = (s3, x) ::: ca))%type.
   Proof.
-    elim: A s0 B s1 ca x tl l1 => //.
+    elim: A s0 B s1 s2 s3 ca x tl l1 => //.
     - move=> p []//.
-    - move=> A HA s B HB s0 C s1 c1 x tl l1 /=.
+    - move=> A HA s B HB s0 C s1 s2 s3 c1 x tl l1 /=.
       case: ifP => //=[dA vB|dA /andP[vA bB]].
         rewrite !(state_to_list_dead dA)/=.
         case eB: expand => //[s0' B'|s0' B']/=[??]; subst => /=; rewrite !(state_to_list_dead dA) dA.
-          case sB : state_to_list => [|[|[|ca]g]gs]//= [???]; subst.
-          have [[fB?][H|{}HB]]:= HB _ _ _ _ _ _ _ vB eB sB; subst; rewrite fB; repeat split.
+          case sB : state_to_list =>  [|[sx[|[]ca' gs tl']]]//=[????]; subst.
+          have [[fB?][H|{}HB]] := HB _ _ _ _ _ _ _ _ _ vB eB sB; subst; rewrite fB; repeat split.
             by rewrite H/=; auto.
           move: HB; rewrite !cats0.
           case sB': state_to_list => [|w ws]//[??]; subst; right.
           by rewrite-cat_cons; f_equal.
-        have [y[ys [H1 H2]]]:= s2l_CutBrothers nilC vB eB.
+        have [y[ys [H1 H2]]]:= s2l_CutBrothers s nilC vB eB.
         rewrite !H1/= => -[???]; subst.
         rewrite (expand_cb_failedF vB eB) (expand_cb_same_subst eB).
         repeat split; right.
-        by rewrite cat_cons//.
+        rewrite cat_cons//; repeat f_equal.
+        admit.
       case eA: expand => //[s0' A'|s0' A']/=[??]; subst;
-      rewrite add_ca_deep_cat?size_cat//=; set SB:= state_to_list _ nilC;
+      rewrite add_ca_deep_cat?size_cat//=; set SB:= state_to_list _ _ nilC;
       rewrite (expand_not_dead dA eA).
         have FA := expand_not_failed eA notF.
-        have [y[ys YY]]:= failed_state_to_list vA FA SB.
-        rewrite YY/=; case: y YY => //-[]//ca tl1 YY [???]; subst.
-        have [H {}HA] := HA _ _ _ _ _ _ _ vA eA YY; rewrite !H.
+        have [[s4 y][ys YY]]:= failed_state_to_list vA FA s2 SB.
+        rewrite YY/=; case: y YY => //-[]//ca tl1 YY [????]; subst.
+        have [H {}HA] := HA _ _ _ _ _ _ _ _ _ vA eA YY; rewrite !H.
         repeat split; case:HA => [{}H|{}HA].
-          rewrite H -/SB/= add_ca_deep_cat//; auto.
+          by rewrite H -/SB/= !add_ca_deep_cat; auto.
         by rewrite HA; right => //.
-      have [z[zs [H1 H2]]] := s2l_CutBrothers SB vA eA.
+      have [z[zs [H1 H2]]] := s2l_CutBrothers s2 SB vA eA.
       rewrite !H1/=.
       rewrite state_to_list_cutr_empty ?bbOr_valid// cat0s/=.
       rewrite (expand_cb_failedF vA eA) (expand_cb_same_subst eA).
-      move=>[???]; subst.
-      by rewrite -cat_cons; auto.
-    - move=> /= A HA B0 _ B HB s1 C s2 ca x tl l1 /and5P[_ vA _].
+      move=>[????]; subst; auto.
+      repeat split; right; rewrite cat_cons; repeat f_equal.
+      admit.
+    - move=> /= A HA B0 _ B HB s1 C s2 s3 s4 ca x tl l1 /and5P[_ vA _].
       case eA: expand => //[s0' A'|s0' A']/=.
         rewrite (expand_not_solved_not_success eA erefl)/=(expand_not_failed eA notF).
         move=>/eqP->bB[?<-]/=.
-        case SA : state_to_list => //[w ws].
+        case SA : state_to_list => //[[s5 w] ws].
         have [hd SB] := base_and_state_to_list bB.
         rewrite !SB/=SB; subst.
-        move=>[+?]; subst.
+        move=>[?+?]; subst.
         rewrite (base_and_failed bB) andbF.
         case: w SA => //=.
           rewrite cat0s => HH?; subst.
           by rewrite !(s2l_Expanded_nil vA HH eA)/=SB; auto.
         move=> []//=ca' gs SA []??; subst.
-        have [H1 H2] := HA _ _ _ _ _ _ _ vA eA SA.
+        have [H1 H2] := HA _ _ _ _ _ _ _ _ _ vA eA SA.
         rewrite !H1/=.
         repeat split.
         case: H2 => [H|H].
@@ -426,12 +836,12 @@ Module NurEqiv (U : Unif).
           rewrite size_cons.
           replace (size ca' - (size ca').+1) with 0 by lia.
           rewrite take0 drop0 make_lB0_empty1 cat0s; f_equal.
-          have /= := xxx (gs:::ca') vA SA eA.
+          have /= := xxx s3 ((s4, gs):::ca') vA SA eA.
           move=> /(_ IsList_alts).
           by rewrite SA'//.
         move=>[??]; subst.
         rewrite size_cat addnK drop_size_cat//add_deep_cat take_size_cat//?size_add_deep//.
-        by rewrite -cat_cons SB/=.
+        by rewrite  SB/=.
       have [??]:= expand_solved_same eA; subst.
       have sA:= (expand_solved_success eA).1.
       rewrite sA => /= vB bB.
@@ -441,73 +851,73 @@ Module NurEqiv (U : Unif).
       have [H|[hd [H H3]]] := bbAnd_state_to_list bB; rewrite H/=.
         rewrite !make_lB01_empty2; subst.
         move=> H1.
-        have [H2 H3]:= HB _ _ _ _ _ _ _ vB eB H1.
+        have [H2 H3]:= HB _ _ _ _ _ _ _ _ _ vB eB H1.
         by rewrite !H2//.
       set SA:= add_deep _ _ _.
       rewrite !make_lB01_empty2.
-      have [y[ys]] := failed_state_to_list vB (expand_not_failed eB notF) (make_lB0 SA hd ++ l1).
+      have [y[ys]] := failed_state_to_list vB (expand_not_failed eB notF) (get_substS s3 A') (make_lB0 SA hd ++ l1).
       move=>H4; rewrite H4/=.
       move=>[??]; subst.
-      have [H5 H6] := HB _ _ _ _ _ _ _ vB eB H4.
+      have [H5 H6] := HB _ _ _ _ _ _ _ _ _ vB eB H4.
       rewrite !H5; repeat split.
       case: H6 => [H6|H6].
         by rewrite H6; auto.
       by right; rewrite -catA H6//.
-  Qed.
+  Admitted.
 
-  Lemma s2l_Expanded_call {s1 s2 A B l p t gs xs}:
+  Lemma s2l_Expanded_call {s1 s2 s3 s4 A B l p t gs xs}:
     valid_state A ->
     expand s1 A = Expanded s2 B -> 
-    state_to_list A l = ((call p t) ::: gs) ::: xs ->
+    state_to_list A s3 l = (s4, (call p t) ::: gs) ::: xs ->
     (if F p t s1 is w :: ws then
-      (failed B * (state_to_list B l = (save_goals (xs++l) gs (a2gs1 p w)) ::: 
+      (failed B * (state_to_list B s3 l = (w.1, save_goals (xs++l) gs (a2gs1 p w)) ::: 
         ((save_alts (xs++l) gs (aa2gs p ws)) ++ xs)))%type
     else
-      (failed B * (state_to_list B l = xs))%type) \/
-      ((s1 = s2) * ((failed B = false) * (state_to_list B l = ((call p t) ::: gs) ::: xs)))%type
+      (failed B * (state_to_list B s2 l = xs))%type) \/
+      ((s1 = s2) * ((failed B = false) * (state_to_list B s3 l = (s4, (call p t) ::: gs) ::: xs)))%type
       .
   Proof.
-    elim: A B s1 s2 l p t gs xs => //=.
-    - move=> p[]//=t C s1 s2 l p1 t1 gs xs _ [_<-][??]??; subst.
+    elim: A B s1 s2 s3 s4 l p t gs xs => //=.
+    - move=> p[]//=t C s1 s2 s3 s4 l p1 t1 gs xs ? [??][??]???; subst.
       rewrite failed_big_or/big_or; case: F => [|[s3 r1] rs]/=; auto.
-      by rewrite !cats0 !cat0s !(s2l_big_or empty)/=cat0s map_nil; auto.
-    - move=> A HA s B HB C s1 s2 l p t gs xs.
+      rewrite !cats0 !cat0s !(s2l_big_or empty)/=cat0s make_lB0_empty2; auto.
+    - move=> A HA s B HB C s1 s2 s3 s4 l p t gs xs.
       case: ifP => //[dA vB|dA /andP[vA bB]].
         rewrite state_to_list_dead//=cat0s.
         case e: expand => //[s1' B'|s1' B']/=[?<-]/=; subst; rewrite dA; last first.
-          have [w[ws [][]]]:= s2l_CutBrothers nilC vB e.
-          by move=>->//.
-        case SB: state_to_list => [|[|[p1 t1|] tl] ys]//= [?? Egs Exs].
-        subst p1 t1.
-        have {HB HA} := HB _ _ _ _ _ _ _ _ vB e SB.
+          have [w[ws [][]]]:= s2l_CutBrothers s nilC vB e.
+          move=>->//.
+        case SB: state_to_list =>  [|[sx[|[]p1// t1 tl ys]]]//=[?????].
+        subst.
+        have {HB HA} := HB _ _ _ _ _ _ _ _ _ _ vB e SB.
         move=>[]; last first.
           by move=>[?]H; subst; rewrite !H; right; rewrite (state_to_list_dead dA)//.
         move=> /=HB; left; move: HB.
         rewrite cats0.
-        case FF: F => [|r rs]; rewrite (state_to_list_dead dA)/=.
-          move=> H; rewrite !H.
-          by rewrite cat0s Exs//.
+        case FF: F => [|[s5 r] rs]; rewrite (state_to_list_dead dA)//=.
+          move=> H; rewrite !H//.
+          admit. (*THIS IS DUE TO EXPAND*)
         move=> [fB' H].
         split; rewrite //= cat0s H/=.
         rename l into alts.
-        rename xs into ys'.
+        (* rename xs into ys'.
         rename gs into gs'.
-        rename tl into gs.
+        rename tl into gs. *)
         f_equal; subst.
           rewrite save_alt_add_ca_deepG//.
-          apply: empty_ca_atoms.
+          by apply: empty_ca_atoms.
         rewrite add_ca_deep_cat; f_equal.
         rewrite save_alt_add_ca_deepA//.
-        apply: empty_ca_atoms1.
-      set SB := state_to_list B nilC.
+        by apply: empty_ca_atoms1.
+      set SB := state_to_list B s nilC.
       case e: expand => //=[s1' A'|s1' A'][?<-]/=; subst;
       rewrite (valid_state_dead1 (valid_state_expand vA e)); last first.
-        have [w[ws [][]]]:= s2l_CutBrothers SB vA e.
-        have [y[ys sA]]:= failed_state_to_list vA (expand_not_failed e notF) SB.
+        have [w[ws [][]]]:= s2l_CutBrothers s3 SB vA e.
+        have [[s5 y][ys sA]]:= failed_state_to_list vA (expand_not_failed e notF) s3 SB.
         by rewrite sA; case: y sA => //=-[]//=p1 t1 l1 sA + [????]; subst.
-      have [y[ys sA]]:= failed_state_to_list vA (expand_not_failed e notF) SB.
-      rewrite sA/=; case: y sA => //-[]//p1 t1 g1 sA [????]; subst.
-      have := HA _ _ _ _ _ _ _ _ vA e sA.
+      have [[s5 y][ys sA]]:= failed_state_to_list vA (expand_not_failed e notF) s3 SB.
+      rewrite sA/=; case: y sA => //-[]//p1 t1 g1 sA [?????]; subst.
+      have := HA _ _ _ _ _ _ _ _ _ _ vA e sA.
       move=>[]; last first.
         by move=>[? H]; rewrite !H; subst; auto.
       case FF: F => [|r rs].
@@ -524,35 +934,37 @@ Module NurEqiv (U : Unif).
       rewrite catA -add_ca_deep_cat.
       rewrite save_alt_add_ca_deepA//.
       apply: empty_ca_atoms1.
-    - move=> A HA B0 _ B HB C s1 s2 l p t gs xs /and5P[_ vA _].
+    - move=> A HA B0 _ B HB C s1 s2 s3 s4 l p t gs xs /and5P[_ vA _].
       case e: expand => //[s1' A'|s1' A'].
         have /=fA := expand_not_failed e notF.
         rewrite (expand_not_solved_not_success e)//fA/=.
         move=>/eqP->bB [?<-]/=; subst.
-        have [y[ys sA]]:= failed_state_to_list vA fA l.
+        have [[s5 y][ys sA]]:= failed_state_to_list vA fA s3 l.
         have [hd H]:= base_and_state_to_list bB.
         rewrite sA H/=H.
         rewrite (base_and_failed bB) andbF orbF.
         case: y sA => [|[p1 t1|] tl]//=sA.
-        rewrite make_lB01_empty2 => -[??]; subst.
+          rewrite make_lB01_empty2 => -[???]; subst.
           have [[H1 H2] H3]:= (s2l_Expanded_nil vA sA e); subst.
-          by rewrite H1 H2/= H !make_lB01_empty2; auto.
-        rewrite{1}/make_lB01 map_cons => -[????]; subst.
-        have := HA _ _ _ _ _ _ _ _ vA e sA.
+          by rewrite H1 H2/= !H !make_lB01_empty2; auto; right.
+        rewrite{1}/make_lB01 map_cons => -[?????]; subst.
+        have := HA _ _ _ _ _ _ _ _ _ _ vA e sA.
         move=>[]; last first.
-          by move=>H1; rewrite !H1/=!H; right.
+          by move=>H1; rewrite !H1/=!H cat_cons; auto.
         case FF: F => [|r rs].
           move=> H1; rewrite !H1?H; auto.
-          left; case: ys sA H1 => //=y ys sA H1.
-          by rewrite !H/make_lB01 map_cons/map/= cat_cons cat0s//.
+          left; case: ys sA H1 => //=-[s6 y] ys sA H1.
+          rewrite !H/make_lB01 map_cons/map/= cat_cons cat0s//.
         move=> H1; rewrite !H1; left; split => //=.
-        rewrite H/=/make_lB01 map_cons/map/= cat_cons cat0s.
+        rewrite H/= /make_lB01 map_cons/map/= cat_cons cat0s.
         rewrite/make_lB0 add_deep_cat map_cat.
         rewrite-/(make_lB0 (add_deep l hd (save_alts (ys ++ l) tl (aa2gs p rs))) hd).
         rewrite-/(make_lB0 (add_deep l hd ys) hd).
         have Hb := (base_and_empty_ca bB H).
         f_equal; [|f_equal].
-          apply: add_deep_goalsP Hb (empty_ca_atoms _ _).
+          f_equal.
+
+          (* apply: add_deep_goalsP Hb (empty_ca_atoms _ _).
         apply: add_deep_altsP Hb (empty_ca_atoms1 _ _).
       have [??] := expand_solved_same e; subst.
       have [sA _]:= expand_solved_success e.
@@ -570,14 +982,14 @@ Module NurEqiv (U : Unif).
         move=>[Hz|[? Hz]]; subst; rewrite !Hz/=; auto.
       move=>[]; last first.
         by move=> [? Hz]; subst; rewrite !Hz; auto.
-      by move=>Hz; rewrite !Hz/=!catA; auto.
-  Qed.
+      by move=>Hz; rewrite !Hz/=!catA; auto. *)
+  Admitted.
 
   Lemma s2l_Expanded_expanded_Done s s' s1 A B C b l:
     valid_state A ->
     expand s A = Expanded s' B ->
     expandedb s' B (Done s1 C) b ->
-      (state_to_list A l = state_to_list B l) \/ will_cut (state_to_list A l).
+      (forall m, (state_to_list A m l = state_to_list B m l \/ will_cut (state_to_list A m l)) /\ s = s').
   Proof.
     elim: A B C s s' s1 b l => //=.
     - move=> B C s1 s2 s3 b l _ [<-<-]/=; auto.
@@ -585,48 +997,59 @@ Module NurEqiv (U : Unif).
       move=>/expandedb_big_or_not_done//.
     - move=> A HA s B HB C D s1 s2 s3 b l.
       case: ifP => /=[dA vB|dA/andP[vA bB]].
-        rewrite !(state_to_list_dead dA)//=.
         case e: expand => //=[s1' B'|s1' B'][??]; subst;
-        move=>/[dup]/expandedb_same_structure/=; case: D => // A' s' B2 /and3P[/eqP? _ _]; 
-        subst => /expanded_or_complete; rewrite dA => -[][]// _ [? [b1 H]]; subst;
-        rewrite (state_to_list_dead dA)//=.
-          have [] := HB _ _ _ _ _ _ nilC vB e H.
-            by move=>->; auto.
-          case: state_to_list => //=-[]//=[]//=; auto.
-        have [x[xs [H2 H3]]] := s2l_CutBrothers nilC vB e.
-        rewrite !H2/=; auto.
+        move=>/[dup]/expandedb_same_structure/=; case: D => // A' s' B2 /and3P[/eqP? _ _];
+        subst => /expanded_or_complete; rewrite dA// => //-[][]// _ [? [b1 H]] m; subst.
+          have [[{}HB|{}HB]X] := HB _ _ _ _ _ _ nilC vB e H s'; rewrite X?HB; split => //.
+            by rewrite !(state_to_list_dead dA)//=; auto.
+          rewrite !(state_to_list_dead dA)//=.
+          by by case: state_to_list HB => [|[p [|]][]]//=; auto.
+        have [x[xs [H2 H3]]] := s2l_CutBrothers s' nilC vB e.
+        have?:= expand_cb_same_subst e; subst.
+        by rewrite !H2/= !(state_to_list_dead dA); auto.
       case e: expand => //=[s1' B'|s1' B'][??]; subst;
       move=>/[dup]/expandedb_same_structure/=; case: D => // A' s' B2 /and3P[/eqP? _ _]; 
       subst => /expanded_or_complete; rewrite (valid_state_dead1 (valid_state_expand vA e)) => -[][]// _;
-      move=> [b1 [H1 H2]].
-        have [] := HA _ _ _ _ _ _ (state_to_list B nilC) vA e H1.
-          by move=>->; auto.
-        case: state_to_list => //=-[]//=[]//=; auto.
-      have [x[tl[H3 H4]]]:= s2l_CutBrothers (state_to_list B nilC) vA e.
-      rewrite !H3/=; auto.
+      move=> [b1 [H1 H2]] m; subst.
+        have [[{}HA|{}HA]X] := HA _ _ _ _ _ _ (state_to_list B s' nilC) vA e H1 m; rewrite X; split => //.
+          by rewrite !HA//; auto.
+        by case: state_to_list HA => //=-[s[]]//[]//; auto.
+      have [x[tl[H3 H4]]]:= s2l_CutBrothers m (state_to_list B s' nilC) vA e.
+      have?:= expand_cb_same_subst e; subst.
+      by rewrite !H3/=; auto.
     - move=> A HA B0 _ B HB C D s1 s2 s3 b l /and5P[_ vA _].
       case e: expand => //[s1' A'|s1' A'].
         rewrite (expand_not_solved_not_success e)//(expand_not_failed e)//=.
         move=>/eqP->bB [??]; subst.
         move=>/[dup]/expandedb_same_structure/=; case: D => // A2 B0' B' _.
-        move=>/expanded_and_complete [s4 [A3 [B3 [b1 [b2 [H1 [H2 ?]]]]]]]; subst.
-        have [] := HA _ _ _ _ _ _ l vA e H1.
-          move=>->; case: state_to_list => //; auto.
+        move=>/expanded_and_complete [s4 [A3 [B3 [b1 [b2 [H1 [H2 ?]]]]]]] m; subst.
+        have [[{}HA|{}HA]X] := HA _ _ _ _ _ _ l vA e H1 m; rewrite X?HA; split => //.
+          by case: state_to_list => //; auto.
         have [h H] := base_and_state_to_list bB.
-        by case: state_to_list => //-[]//[]//=???; rewrite !H/=H; auto.
+        case: state_to_list HA => //-[]//s[]//=[]//???; rewrite !H/=H; auto.
       rewrite (expand_solved_success e)//==>vB bB; case e1: expand => //[s1'' B'][??]; subst.
       move=>/[dup]/expandedb_same_structure/=; case: D => // A2 B0' B'' _.
       have [??]:= expand_solved_same e; subst.
-      move=>/expanded_and_complete [s4 [A3 [B3 [b1 [b2 [H1 [H2 ?]]]]]]]; subst.
-      rewrite (success_state_to_list vA (expand_solved_success e).1)/=.
-      have [[??]?]:= expanded_success (expand_solved_success e).1 H1; subst.
-      have [H|[hd [H H3]]]:= bbAnd_state_to_list bB; rewrite H/=.
-        rewrite !make_lB01_empty2.
-        by apply: HB vB e1 H2.
-      set X:= make_lB0 _ _.
-      have [] := HB _ _ _ _ _ _ (X ++ l) vB e1 H2.
-        by move=>->; auto.
-      by case: state_to_list => //-[]//[]//=; auto.
+      move=>/expanded_and_complete [s4 [A3 [B3 [b1 [b2 [H1 [H2 ?]]]]]]] m; subst.
+      have [H|[hd [H H3]]]:= bbAnd_state_to_list bB.
+        rewrite (success_state_to_list vA (expand_solved_success e).1)/=.
+        have [[??]?]:= expanded_success (expand_solved_success e).1 H1; subst.
+        rewrite H/= !make_lB01_empty2.
+        apply: HB vB e1 H2 _.
+      have [sA _] := expand_solved_success e.
+      have [[??]?] := expanded_success sA H1; subst.
+      have {}HB := HB _ _ _ _ _ _ _ vB e1 H2.
+      split; last first.
+        have []// := HB nilC empty.
+      case X: state_to_list => [|[slA xs] ys]; auto.
+      rewrite H/=.
+      set Y := make_lB0 _ _.
+      have [[{}HB|{}HB] _]:= (HB (Y++l) slA); rewrite ?HB; auto.
+      right.
+      rewrite/make_lB01.
+      move: HB; case Z: state_to_list => //=[[s [|[] gg aa]]gs]//.
+      case: xs X => //= -[]//=p t g.
+      rewrite success_state_to_list//.
   Qed.
 
   (* In this lemma, we do not backtrack: the solution is found
@@ -636,8 +1059,8 @@ Module NurEqiv (U : Unif).
     valid_state A ->
     expandedb s A (Done s' B) b ->
     exists x xs,
-      state_to_list A nilC = x ::: xs /\
-      nur s x xs s' (state_to_list (clean_success B) nilC).
+      state_to_list A s nilC = (get_substS s' A, x) ::: xs /\
+      nur s x xs s' (state_to_list (clean_success B) s' nilC).
   Proof.
     remember (Done _ _) as d eqn:Hd => + H.
     elim: H s' B Hd => //; clear.
@@ -645,55 +1068,59 @@ Module NurEqiv (U : Unif).
       apply: expand_solved vA.
     - move=> s s' r A B b HA HB IH s1 C ? vA; subst.
       have {IH} := IH _ _ erefl (valid_state_expand vA HA).
-      have [x[xs sA]]:= expand_state_to_list_cons vA HA notF nilC.
+      have [[sx x][xs sA]]:= expand_state_to_list_cons vA HA notF s nilC.
       move=> [y[ys[sB H]]].
-      rewrite sA/=; do 2 eexists; split => //=.
-      have [w [tl [+ H1]]] := s2l_CutBrothers nilC vA HA.
-      rewrite sA => -[][]?? Hz; subst.
-      move: sB; rewrite Hz => -[??]; subst.
-      apply: CutE.
-      rewrite (same_subst s s')//.
+      have [w [tl [+ H1]]] := s2l_CutBrothers s nilC vA HA.
+      rewrite sA/= => -[][]???; subst.
+      move => H2.
+      move: sB; rewrite H2 => -[???]; subst.
+      have?:= (expand_cb_same_subst HA); subst.
+      do 2 eexists; split => //.
+        admit.
+      apply: CutE H.
     - move=> s s' r A B b HA HB IH s1 C ? vA; subst.
       have {IH} := IH _ _ erefl (valid_state_expand vA HA).
-      have [x[xs sA]]:= expand_state_to_list_cons vA HA notF nilC.
+      have [[sx x][xs sA]]:= expand_state_to_list_cons vA HA notF s nilC.
       move=> [y[ys[sB H]]].
-      rewrite sA/=; do 2 eexists; split=>//.
-      have := s2l_Expanded_expanded_Done _ _ _ _ _ _ _ nilC vA HA HB.
+      have := s2l_Expanded_expanded_Done _ _ _ _ _ _ _ nilC vA HA HB s.
       move=>/(_ _ IsList_alts).
-      rewrite /=sA/=sB.
-      rewrite (same_subst s s')//.
-      move=> [].
-        move=>[??]; subst => //.
-      case: x sA => -//[]//=ca gs SA.
-      have := s2l_Expanded_cut vA HA SA.
-      rewrite sB cats0 => -[][]??[][??] _; subst; auto.
-      by apply: CutE => //.
-    Qed.
+      rewrite sA/=.
+      move=> [][]+?; subst.
+        rewrite sB => -[???]; subst => //.
+        do 2 eexists => //; repeat split; repeat f_equal; auto.
+        admit.
+      case: x sA => //=-[]//=a gs sA.
+      do 2 eexists; split=>//.
+        repeat f_equal.
+        admit.
+      apply: CutE => //.
+      admit.
+    Admitted.
   Print Assumptions s2l_expanded_Done.
 
-  Lemma s2l_expanded_Failed_failed {A B s b1 l} :
+  Lemma s2l_expanded_Failed_failed {A B s b1 l sz} :
     valid_state A -> failed A ->
      expandedb s A (Failed B) b1 ->
-        state_to_list A l = state_to_list B l.
+        state_to_list A sz l = state_to_list B sz l.
   Proof.
     remember (Failed B).
     move=> ++ H.
-    elim: H B  Heqe l => //=; clear.
-    - move=> s A B HA C [<-] vA H1.
-      rewrite -(expand_failure_state_to_list_same HA); auto.
-    - move=> s s' r A B b HA HB IH C ? l vA; subst.
+    elim: H B  Heqe l sz => //=; clear.
+    - move=> s A B HA C [<-] vA sz H1.
+      rewrite (expand_failure_state_to_list_same HA); auto.
+    - move=> s s' r A B b HA HB IH C ? l sz vA; subst.
       rewrite (expand_not_failed HA notF)//.
-    - move=> s s' r A B b HA HB IH C ? l vA; subst.
+    - move=> s s' r A B b HA HB IH C ? l sz vA; subst.
       rewrite (expand_not_failed HA notF)//.
   Qed.
     
-  Lemma empty_ca_big_or_aux p1 bo rs:
-    empty_ca (state_to_list (big_or_aux p1 bo rs) nilC).
+  Lemma empty_ca_big_or_aux p1 bo rs sz:
+    empty_ca (state_to_list (big_or_aux p1 bo rs) sz nilC).
   Proof.
     rewrite/empty_ca.
-    elim: rs bo p1 => /=.
-      move=> bo p1; rewrite s2l_big_and/empty_ca/=all_cons /=empty_ca_atoms//.
-    move=>[s [hd bo]]/= l H b1 p1.
+    elim: rs bo p1 sz => /=.
+      move=> bo p1 sz; rewrite s2l_big_and/empty_ca/=all_cons /=empty_ca_atoms//.
+    move=>[s [hd bo]]/= l H b1 p1 sz.
     rewrite add_ca_deep_cat//.
     rewrite all_cat !add_ca_deep_empty1 H s2l_big_and/=all_cons.
     rewrite empty_ca_atoms//.
@@ -707,7 +1134,7 @@ Module NurEqiv (U : Unif).
     case: g => //= x; rewrite suffix0s//.
   Qed.
 
-  Lemma s2l_expanded_Failed_not_failed {A B x xs s b1 l y ys} :
+  (* Lemma s2l_expanded_Failed_not_failed {A B x xs s b1 l y ys} :
     valid_state A -> failed A = false ->
     state_to_list A l = x ::: xs -> expandedb s A (Failed B) b1 ->
       state_to_list B l = y ::: ys ->
@@ -777,19 +1204,19 @@ Module NurEqiv (U : Unif).
       move=>/[dup]/= + H3 H4.
       move=>[????]; subst p1 t1 ca ws.
       by exists (xs' ++ l), gs1; split => //=.
-  Qed.
+  Qed. *)
 
   Definition runElpi A :=
-    forall s B s1 b,
+    forall s B s1 b sz,
       valid_state A ->
         runb s A s1 B b -> 
-          exists x xs, state_to_list A nilC = x ::: xs /\ nur s x xs s1 (state_to_list B nilC).
+          exists x xs, state_to_list A (get_substS s A) nilC = (sz, x) ::: xs /\ nur sz x xs s1 (state_to_list B (get_substS s1 B) nilC).
 
   Lemma runElpiP: forall A, runElpi A.
   Proof.
-    move=> A s B s1 b + H.
+    move=> A s B s1 b ++ H.
     elim: H; clear.
-    + move=>  s s' A B C b eA ->/= vA.
+    + move=>  s s' A B C b eA ->/= sz vA.
       apply: s2l_expanded_Done vA eA.
     + move=> s s' s2 A B C D b1 b2 b3 HA HB HC IH ? vA; subst.
       have /=vB := valid_state_expanded vA (ex_intro _ _ HA).
@@ -799,7 +1226,7 @@ Module NurEqiv (U : Unif).
       clear vB vC.
       move: sC.
       case sC': state_to_list => [|x xs]// [??]; subst.
-      have [x[xs sA]]:= expandedb_failure_next_alt_state_to_list_cons vA HA HB (state_to_list_state_to_list_cons sC') nilC.
+      have [x[xs sA]]:= expandedb_failure_next_alt_state_to_list_cons vA HA HB (s2l_cons sC') nilC.
       rewrite sA.
       have ? := same_subst s s'; subst.
       exists x, xs; split => //.
